Replace BitVector with Integers from CompCert

Isa/Val.v
@@ -1,5 +1,5 @@
 Require Import Arith Util EqDec List.
-Require Import OrderedTypeEx BitVector.
+Require Import OrderedTypeEx Integers.
 
 Set Implicit Arguments.
 
@@ -7,65 +7,49 @@ Set Implicit Arguments.
 (** A file that abstacts over values and (should) provide all necessary operations. Although we concretely instantiate val to int, we maintain this file as interface between our proofs and Integer library. *)
 
 (** Make the value type bitvectors and the default value 0 as a bitvector **)
-Definition val := bitvec.
-Definition default_val : val := (zext (O::nil)).
+Definition val := int.
+Definition default_val : val := Int.zero.
 
-Opaque val.
-Opaque default_val.
-
-(** Default value for true = 1 = 2^1 , false = 0 = 2^0 **)
-Definition val_true := (sext (I::nil) I).
-Definition val_false := (zext (O::nil)).
-
-Fixpoint eqValList (l1:list bitvec) (l2:list bitvec) :=
-match l1, l2 with
-| nil, _ => val_false
-| _, nil => val_false
-| a::l1', b::l2' => bvAnd (eqValList l1' l2') (bvEq a b)
-end.
-
-Global Instance inst_val_defaulted : Defaulted val := {
+Instance inst_val_defaulted : Defaulted val := {
   default_el := default_val
 }.
 
-Global Instance inst_eq_dec_val : EqDec val eq.
-hnf; intros. change ({x = y} + {x <> y}).
-assert (X:forall b1 b2:bit, {b1 = b2} + {b1 <> b2}).
-- intros. destruct b1, b2.
-  + left; reflexivity.
-  + right; firstorder.
-  + right; firstorder.
-  + left; reflexivity.
-- exact (list_eq_dec X x y).
+(** Default value for true = 1 = 2^1 , false = 0 = 2^0 **)
+Definition val_true := Int.one.
+Definition val_false := Int.zero.
+Lemma val_true_false_neq
+  : val_true <> val_false.
+Proof.
+  eapply Int.one_not_zero.
+Qed.
+
+Definition val_zero : val := Int.zero.
+
+Instance inst_eq_dec_val : EqDec val eq.
+hnf; intros. eapply Int.eq_dec.
 Defined.
 
 (** ** There must be an injection into the booleans *)
-Definition val2bool : val -> bool := fun v => toBool  v. (*  match v with 0 => false | _ => true end. *)
+Definition val2bool (v: val) : bool := if [ v = val_zero ] then false else true.
 
 Lemma val2bool_true
 : val2bool val_true = true.
 Proof.
-  unfold val_true, val2bool, sext.
-  rewrite toBool_I_true; [auto|].
-  pose proof K_ge1; auto.
+  unfold val2bool.
+  cases; eauto.
+  exfalso; eauto using val_true_false_neq.
 Qed.
 
 Lemma val2bool_false
 : val2bool val_false = false.
 Proof.
-  unfold val2bool, val_false, zext.
-  rewrite toBool_O_false; auto.
+  unfold val2bool.
+  cases; eauto.
 Qed.
 
+Opaque val.
+Opaque default_val.
+Opaque val_true.
+Opaque val_false.
+Opaque val_zero.
 Opaque val2bool.
-
-Inductive ty : Set :=
-  Natural : ty.
-
-Global Instance inst_eq_dec_ty : EqDec ty eq.
-hnf; intros. change ({x = y} + {x <> y}).
-decide equality.
-Defined.
-
-Inductive valOfType : val -> ty -> Prop :=
-  naturalOfType n : valOfType n Natural.
